src/InvariantsTactics.v
@@ -18,7 +18,7 @@
   Foundation, Inc., 51 Franklin St, Fifth Floor, Boston, MA  02110-1301 USA *)
 
 Set Implicit Arguments.
-From TLC Require Import LibCollection.
+From TLC Require Import LibContainer.
 From Paco Require Import paco.
 Require Import InvariantsAux.
 
